DependentComputability/Tactic/DCompHelperLemmas.lean
@@ -1,0 +1,99 @@
+import DependentComputability.DComp
+import DependentComputability.Tactic.ConvertToNew
+
+open Lean Meta Qq
+
+set_option backward.do.legacy false
+
+namespace DCompHelperTheorems
+
+def withManyDependentSorts (n : Nat)
+    (k : (u : Level) → Q(Sort u) → Array Expr → MetaM α) : MetaM α :=
+  match n with
+  | 0 => unreachable!
+  | k + 1 =>
+    have u_1 : Level := .param `u_1
+    withLocalDeclQ `α_1 .implicit q(Sort u_1) fun var => do
+      go k _ q($var) #[var]
+where
+  go (n : Nat) (lastUniv : Level) (lastType : Q(Sort lastUniv)) (acc : Array Expr) : MetaM α :=
+    match n with
+    | 0 => k lastUniv lastType acc
+    | n + 1 =>
+      have v : Level := .param <| (`u).appendIndexAfter (acc.size + 1)
+      let ty := q($lastType → Sort v)
+      withLocalDeclQ ((`α).appendIndexAfter (acc.size + 1)) .implicit ty fun var =>
+        go n _ q(PSigma $var) (acc.push var)
+
+def mkBVarLemma (comp : Bool) (priv : Bool) (last : Bool) (n : Nat) : MetaM Name := do
+  let root := if comp then ``DComp else ``DPrim
+  let baseName := root ++ if last then `bvar_last else `bvar_before
+  let baseName := baseName.appendIndexAfter n
+  if (← getEnv).contains baseName then
+    return baseName
+  let privName := mkPrivateName (← getEnv) baseName
+  if (← getEnv).contains privName then
+    return privName
+  let prevLemma ←
+    if comp then
+      mkBVarLemma false priv last n
+    else if last then
+      if n = 0 then
+        unreachable!
+      else
+        mkBVarLemma comp priv true (n - 1)
+    else
+      mkBVarLemma comp priv true n
+  let name := if priv then privName else baseName
+  let nvars := if last then n + 1 else n + 2
+  withManyDependentSorts nvars fun u ctx types => do
+    have v : Level := if last then .param `u_1 else .param `u_2
+    let proj : Expr := n.repeat (.proj ``PSigma 0) (.bvar 0)
+    let projTy : Expr := if last then types[0]! else .app types[1]! (.proj ``PSigma 0 proj)
+    let proj := if last then proj else .proj ``PSigma 1 proj
+    have projTy : Q($ctx → Sort v) := .lam `c ctx projTy .default
+    have projFn : Q((c : $ctx) → $projTy c) := .lam `c ctx proj .default
+    let us := List.ofFn fun i : Fin nvars => .param <| (`u).appendIndexAfter (i + 1)
+    if comp then
+      let type := q(DComp $projFn)
+      have proof : Q(DPrim $projFn) := mkAppN (.const prevLemma us) types
+      let proof : Q(DComp $projFn) := q(.of_prim $proof)
+      addDecl <| .thmDecl {
+        name,
+        levelParams := List.ofFn fun i : Fin nvars => (`u).appendIndexAfter (i + 1)
+        type := ← mkForallFVars types type,
+        value := ← mkLambdaFVars types proof
+      }
+      return name
+    let lemmaName := if last then ``PSigma.fst.dprim else ``PSigma.snd.dprim
+    have αu : Level := .param `u_1
+    have βu : Level := .param `u_2
+    have αvar : Q(Sort αu) := types[0]!
+    have βvar : Q($αvar → Sort βu) := types[1]!
+    let newUs := ql(max (max 1 αu) βu) :: us.tail.tail
+    let sigma := q(PSigma $βvar)
+    let proof := mkAppN (.app (.const prevLemma newUs) sigma) (types.drop 2)
+    let proof := mkApp5 (.const lemmaName [u, αu, βu]) ctx
+      q(fun _ : $ctx => $αvar) q(fun _ : $ctx => $βvar)
+      (.lam `c ctx proj.projExpr! .default) proof
+    addDecl <| .thmDecl {
+      name,
+      levelParams := List.ofFn fun i : Fin nvars => (`u).appendIndexAfter (i + 1)
+      type := ← mkForallFVars types q(DPrim $projFn),
+      value := ← mkLambdaFVars types proof
+    }
+    return name
+termination_by if comp then 3 * n + 2 else if last then 3 * n else 3 * n + 1
+decreasing_by all_goals grind
+
+end DCompHelperTheorems
+
+lemma DPrim.bvar_last_0 {α : Sort u} : DPrim fun c : α => c := .id
+lemma DComp.bvar_last_0 {α : Sort u} : DComp fun c : α => c := .id
+
+-- probably as much as you'll ever need
+open DCompHelperTheorems in
+run_meta
+  for i in *...48 do
+    discard <| mkBVarLemma (comp := true) (priv := false) (last := false) i
+    discard <| mkBVarLemma (comp := true) (priv := false) (last := true) i
